Primitive_Matchers/Common_Primitive_Matcher.thy
@@ -1,0 +1,104 @@
+theory Common_Primitive_Matcher
+imports "../Semantics_Ternary" Common_Primitive_Syntax "../Bitmagic/IPv4Addr" "../Unknown_Match_Tacs"
+begin
+
+
+subsection{*Primitive Matchers: IP Port Iface Matcher*}
+
+fun common_matcher :: "(common_primitive, simple_packet) exact_match_tac" where
+  "common_matcher (IIface i) p = bool_to_ternary (match_iface i (p_iiface p))" |
+  "common_matcher (OIface i) p = bool_to_ternary (match_iface i (p_oiface p))" |
+
+  "common_matcher (Src ip) p = bool_to_ternary (p_src p \<in> ipv4s_to_set ip)" |
+  "common_matcher (Dst ip) p = bool_to_ternary (p_dst p \<in> ipv4s_to_set ip)" |
+
+  "common_matcher (Prot proto) p = bool_to_ternary (match_proto proto (p_proto p))" |
+
+  "common_matcher (Src_Ports ps) p = bool_to_ternary (p_sport p \<in> ports_to_set ps)" |
+  "common_matcher (Dst_Ports ps) p = bool_to_ternary (p_dport p \<in> ports_to_set ps)" |
+
+  "common_matcher (Extra _) p = TernaryUnknown"
+
+
+
+  text{*Warning: beware of the sloppy term `empty' portrange*} 
+  text{*An `empty' port range means it can never match! Basically, @{term "MatchNot (Match (Src_Ports [(0,65535)]))"} is False*}
+  lemma "\<not> matches (common_matcher, \<alpha>) (MatchNot (Match (Src_Ports [(0,65535)]))) a 
+          \<lparr>p_iiface = ''eth0'', p_oiface = ''eth1'', p_src = ipv4addr_of_dotteddecimal (192,168,2,45), p_dst= ipv4addr_of_dotteddecimal (173,194,112,111),
+                   p_proto=TCP, p_sport=2065, p_dport=80\<rparr>"
+  (*<*)by(simp add: matches_case_ternaryvalue_tuple split: ternaryvalue.split)(*>*)
+  text{*An `empty' port range means it always matches! Basically, @{term "(MatchNot (Match (Src_Ports [])))"} is True.
+        This corresponds to firewall behavior, but usually you cannot specify an empty portrange in firewalls, but omission of portrange means no-port-restrictions, 
+        i.e. every port matches.*}
+  lemma "matches (common_matcher, \<alpha>) (MatchNot (Match (Src_Ports []))) a 
+          \<lparr>p_iiface = ''eth0'', p_oiface = ''eth1'', p_src = ipv4addr_of_dotteddecimal (192,168,2,45), p_dst= ipv4addr_of_dotteddecimal (173,194,112,111),
+                   p_proto=TCP, p_sport=2065, p_dport=80\<rparr>"
+  (*<*)by(simp add: matches_case_ternaryvalue_tuple split: ternaryvalue.split)(*>*)
+  text{*If not a corner case, portrange matching is straight forward.*}
+  lemma "matches (common_matcher, \<alpha>) (Match (Src_Ports [(1024,4096), (9999, 65535)])) a 
+          \<lparr>p_iiface = ''eth0'', p_oiface = ''eth1'', p_src = ipv4addr_of_dotteddecimal (192,168,2,45), p_dst= ipv4addr_of_dotteddecimal (173,194,112,111),
+                   p_proto=TCP, p_sport=2065, p_dport=80\<rparr>"
+        "\<not> matches (common_matcher, \<alpha>) (Match (Src_Ports [(1024,4096), (9999, 65535)])) a 
+          \<lparr>p_iiface = ''eth0'', p_oiface = ''eth1'', p_src = ipv4addr_of_dotteddecimal (192,168,2,45), p_dst= ipv4addr_of_dotteddecimal (173,194,112,111),
+                   p_proto=TCP, p_sport=5000, p_dport=80\<rparr>"
+        "\<not>matches (common_matcher, \<alpha>) (MatchNot (Match (Src_Ports [(1024,4096), (9999, 65535)]))) a 
+          \<lparr>p_iiface = ''eth0'', p_oiface = ''eth1'', p_src = ipv4addr_of_dotteddecimal (192,168,2,45), p_dst= ipv4addr_of_dotteddecimal (173,194,112,111),
+                   p_proto=TCP, p_sport=2065, p_dport=80\<rparr>"
+  (*<*)by(simp_all add: matches_case_ternaryvalue_tuple split: ternaryvalue.split)(*>*)
+  
+  
+
+
+
+text{*Lemmas when matching on @{term Src} or @{term Dst}*}
+lemma common_matcher_SrcDst_defined:
+  "common_matcher (Src m) p \<noteq> TernaryUnknown"
+  "common_matcher (Dst m) p \<noteq> TernaryUnknown"
+  "common_matcher (Src_Ports ps) p \<noteq> TernaryUnknown"
+  "common_matcher (Dst_Ports ps) p \<noteq> TernaryUnknown"
+  apply(case_tac [!] m)
+  apply(simp_all add: bool_to_ternary_Unknown)
+  done
+lemma common_matcher_SrcDst_defined_simp:
+  "common_matcher (Src x) p \<noteq> TernaryFalse \<longleftrightarrow> common_matcher (Src x) p = TernaryTrue"
+  "common_matcher (Dst x) p \<noteq> TernaryFalse \<longleftrightarrow> common_matcher (Dst x) p = TernaryTrue"
+apply (metis eval_ternary_Not.cases common_matcher_SrcDst_defined(1) ternaryvalue.distinct(1))
+apply (metis eval_ternary_Not.cases common_matcher_SrcDst_defined(2) ternaryvalue.distinct(1))
+done
+lemma match_simplematcher_SrcDst:
+  "matches (common_matcher, \<alpha>) (Match (Src X)) a p \<longleftrightarrow> p_src  p \<in> ipv4s_to_set X"
+  "matches (common_matcher, \<alpha>) (Match (Dst X)) a p \<longleftrightarrow> p_dst  p \<in> ipv4s_to_set X"
+   apply(simp_all add: matches_case_ternaryvalue_tuple split: ternaryvalue.split)
+   apply (metis bool_to_ternary.elims bool_to_ternary_Unknown ternaryvalue.distinct(1))+
+   done
+lemma match_simplematcher_SrcDst_not:
+  "matches (common_matcher, \<alpha>) (MatchNot (Match (Src X))) a p \<longleftrightarrow> p_src  p \<notin> ipv4s_to_set X"
+  "matches (common_matcher, \<alpha>) (MatchNot (Match (Dst X))) a p \<longleftrightarrow> p_dst  p \<notin> ipv4s_to_set X"
+   apply(simp_all add: matches_case_ternaryvalue_tuple split: ternaryvalue.split)
+   apply(case_tac [!] X)
+   apply(simp_all add: bool_to_ternary_simps)
+   done
+lemma common_matcher_SrcDst_Inter:
+  "(\<forall>m\<in>set X. matches (common_matcher, \<alpha>) (Match (Src m)) a p) \<longleftrightarrow> p_src p \<in> (\<Inter>x\<in>set X. ipv4s_to_set x)"
+  "(\<forall>m\<in>set X. matches (common_matcher, \<alpha>) (Match (Dst m)) a p) \<longleftrightarrow> p_dst p \<in> (\<Inter>x\<in>set X. ipv4s_to_set x)"
+  apply(simp_all)
+  apply(simp_all add: matches_case_ternaryvalue_tuple bool_to_ternary_Unknown bool_to_ternary_simps split: ternaryvalue.split)
+ done
+
+
+
+text{* multiport list is a way to express  disjunction in one matchexpression in some firewalls*}
+lemma multiports_disjuction:
+        "(\<exists>rg\<in>set spts. matches (common_matcher, \<alpha>) (Match (Src_Ports [rg])) a p) \<longleftrightarrow>
+        matches (common_matcher, \<alpha>) (Match (Src_Ports spts)) a p"
+        "(\<exists>rg\<in>set dpts. matches (common_matcher, \<alpha>) (Match (Dst_Ports [rg])) a p) \<longleftrightarrow>
+        matches (common_matcher, \<alpha>) (Match (Dst_Ports dpts)) a p"
+  apply(simp_all add: bool_to_ternary_Unknown matches_case_ternaryvalue_tuple bunch_of_lemmata_about_matches bool_to_ternary_simps split: ternaryvalue.split ternaryvalue.split_asm)
+  apply(simp_all add: ports_to_set)
+  apply(safe) (*ugly proof*)
+     apply force+
+  done
+  
+
+
+end
