Primitive_Matchers/Transform.thy
@@ -1,0 +1,12 @@
+theory Transform
+imports "IPPortIfaceSpace_Matcher"
+        "../Semantics_Ternary"
+        "../Output_Format/Negation_Type_Matching"
+        "../Primitive_Matchers/Ports_Normalize"
+        "../Primitive_Matchers/IpAddresses_Normalize"
+begin
+
+
+
+
+end
